proof/garble/clonesMean.ec
@@ -1,13 +1,14 @@
 require import FSet. import Interval.
+require ISet.
 require import Int.
 require import Bool.
 require import Distr.
 require import Real.
 
-require import Mean. export MReal.SumSet.
+require import Mean.
+require import Monoid. import Mrplus.
 
 require import PreProof.
-
 require import ReductionAda.
 
 lemma DkcExp : forall (M<:DKCS.Exp),
@@ -16,17 +17,40 @@ by (intros _;fun true;progress assumption).
 
 clone Mean as MeanBool with
   type base = bool,
-  op d = Dbool.dbool,
-  op support = add false (add true empty)
-  proof in_support
-  by (intros=> x;delta support d;rewrite ! mem_add;case x=> ? /=;apply Dbool.supp_def).
+  op d = Dbool.dbool.
+op suppBool = add false (add true FSet.empty).
+lemma suppBool : forall x, in_supp x MeanBool.d <=> mem x suppBool
+  by (intros=> x;rewrite /suppBool /MeanBool.d ! mem_add Dbool.supp_def;case x=> ? //).
+lemma mem_suppBool : forall x, ISet.mem x (ISet.support MeanBool.d) <=> mem x suppBool
+  by (intros x;rewrite /ISet.support ISet.mem_create /= suppBool //).
+lemma suppBoolF : ISet.Finite.finite (ISet.support (MeanBool.d))
+  by (exists suppBool=> x;rewrite /ISet.Finite.finite mem_suppBool //).
+lemma suppBoolV : ISet.Finite.toFSet (ISet.support (MeanBool.d)) = suppBool.
+proof strict.
+  apply set_ext=> x.
+  rewrite ISet.Finite.mem_toFSet;
+    first by apply suppBoolF.
+  rewrite mem_suppBool //.
+qed.
+
 
 clone Mean as MeanInt with
   type base = int,
-  op d = Dinter.dinter 0 (Cst.bound-1),
-  op support = interval 0 (Cst.bound-1)
-  proof in_support
-  by (intros=> x;delta support d;rewrite mem_interval Dinter.supp_def //).
+  op d = Dinter.dinter 0 (Cst.bound-1).
+op suppInt = interval 0 (Cst.bound-1).
+lemma suppInt : forall x,in_supp x MeanInt.d <=> mem x suppInt
+  by (intros=> x;rewrite /suppInt mem_interval /MeanInt.d Dinter.supp_def //).
+lemma mem_suppInt : forall x, ISet.mem x (ISet.support MeanInt.d) <=> mem x suppInt
+  by (intros x;rewrite /ISet.support ISet.mem_create /= suppInt //).
+lemma suppIntF : ISet.Finite.finite (ISet.support (MeanInt.d))
+  by  (exists suppInt=> x;rewrite /ISet.Finite.finite /ISet.support ISet.mem_create /= suppInt //).
+lemma suppIntV : ISet.Finite.toFSet (ISet.support (MeanInt.d)) = suppInt.
+proof strict.
+  apply set_ext=> x.
+  rewrite ISet.Finite.mem_toFSet;
+    first by apply suppIntF.
+  rewrite mem_suppInt //.
+qed.
 
 module DkcWork(Adv:DKCS.AdvAda_t) : MeanBool.Worker = {
   module Game = DKCS.GameAda(DKCS.Dkc, Adv)
@@ -76,9 +100,9 @@ save.
 
 lemma DkcEsp :
   forall &m,
-    forall (Adv<:DKCS.AdvAda_t {DKCS.Dkc, DKCS.Game}),
+    forall (Adv<:DKCS.AdvAda_t {DKCS.Dkc, DKCS.Game, MeanBool.Rand}),
       Pr[DKCS.GameAda(DKCS.Dkc, Adv).main()@ &m:res] = 
-        (MReal.(+) Pr[DkcWork(Adv).work(true)@ &m:res]
+        (Mrplus.Base.(+) Pr[DkcWork(Adv).work(true)@ &m:res]
            Pr[DkcWork(Adv).work(false)@ &m:res]) / 2%r.
 proof strict.
   intros &m Adv.
@@ -98,14 +122,11 @@ proof strict.
       call (_:(glob Adv){1} = (glob Adv){2} ==> (glob Adv){1} = (glob Adv){2});first (fun true;by progress).
       wp;rnd;skip;by (progress assumption).
     equiv_deno eq;progress assumption;smt.
-  rewrite pr (MeanBool.Mean &m (DkcWork(Adv))).
-  delta MeanBool.support.
-  (rewrite ! sum_add;first rewrite mem_add /=);first 2 apply mem_empty.
-  rewrite sum_nil /=.
-  delta MeanBool.d.
-  rewrite ! Dbool.mu_x_def MReal.addZ MReal.C /MReal.(+).
-  admit.
-  (*smt.*)
+  rewrite pr (MeanBool.Mean &m (DkcWork(Adv)));first by apply suppBoolF.
+  (rewrite suppBoolV /suppBool ! sum_add;first rewrite mem_add /=);first 2 apply mem_empty.
+  simplify MeanBool.d.
+  rewrite sum_empty ! Dbool.mu_x_def.
+  smt.
 save.
 
 theory RedEsp.
@@ -130,6 +151,7 @@ lemma RemRedEsp : forall (p:bool -> bool) (ADV <: PrvIndSec.Adv_t{RedAda, DKCS.D
   (glob ADV){1} = (glob ADV){2}=>
   Pr[RedWork(ADV).work(l)@ &1:p res] = Pr[PreInit(ADV).f(l, b)@ &2:p res].
 proof strict.
+(*Proof correct but take a lot of useless time*)
 intros=> ? ? ? ? ? ? ? ?;
 (equiv_deno(_: ={glob DKCS.GameAda,glob RedAda,glob ADV}/\
               x{1}=vl{2}/\b=vb{2} ==> ={res});
@@ -139,9 +161,9 @@ save.
 
 lemma AdvEsp :
   forall &m,
-    forall (ADV<:PrvIndSec.Adv_t{DKCS.Dkc,RedAda,DKCS.Game}),
+    forall (ADV<:PrvIndSec.Adv_t{DKCS.Dkc,RedAda,DKCS.Game,MeanInt.Rand}),
       Pr[DkcWork(RedAda(ADV)).work(b)@ &m:res] =
-        (sum (lambda l, (1%r / Cst.bound%r) * Pr[RedWork(ADV).work(l)@ &m:res]) MeanInt.support).
+        (sum (lambda l, (1%r / Cst.bound%r) * Pr[RedWork(ADV).work(l)@ &m:res]) suppInt).
 proof strict.
   intros &m ADV.
   cut <- : (Pr[MeanInt.Rand(RedWork(ADV)).randAndWork()@ &m:res] = Pr[DkcWork(RedAda(ADV)).work(b)@ &m:res]).
@@ -153,13 +175,12 @@ proof strict.
       wp;rnd;wp;skip;progress assumption.
 rewrite sum_in.
 simplify.
-delta MReal.Z.
 cut -> : ((lambda (x:int),
-(if mem x MeanInt.support then Pr[RedWork(ADV).work(x) @ &m : res{hr}]/Cst.bound%r else
-  0%r)) = lambda (x:int), (mu_x MeanInt.d x * Pr[RedWork(ADV).work(x) @ &m :res{hr}]));
-last apply (MeanInt.Mean &m (RedWork(ADV))).
+(if mem x suppInt then Pr[RedWork(ADV).work(x) @ &m : res{hr}]/Cst.bound%r else
+  Z)) = lambda (x:int), (mu_x MeanInt.d x * Pr[RedWork(ADV).work(x) @ &m :res{hr}]));
+last rewrite -suppIntV;apply (MeanInt.Mean &m (RedWork(ADV)));apply suppIntF.
 apply fun_ext=> x /=.
-case (mem x MeanInt.support = true);
+case (mem x suppInt = true);
   [|rewrite rw_eqT -rw_neqF];
   intros=> memX;rewrite memX /=;
   rewrite /MeanInt.d;
